\documentclass{article}
\usepackage{amsmath}

\begin{document}
	
	\section{}
		\subsection{}
		\[
	\lim_{x \to 0} \frac{x^2 - 2x + 1}{x - 1}
	= \lim_{x \to 0}\frac{(x - 1)^2}{x - 1}=
	\lim_{x \to 0}\frac{(x - 1)^2}{x - 1} =\lim_{x \to 0} x - 1=\boxed{-1}
	\]
		\subsection{}
		
			\[	
\lim_{x \to 1} \frac{x^2 - 2x + 1}{x - 1}
= \lim_{x \to 1} \frac{(x - 1)^2}{x - 1}
= \lim_{x \to 1} (x - 1)
= \boxed{0}
\]	
		
		\subsection{}

	\[
\lim_{x \to \infty} \left(1 + \frac{1}{x}\right)\left(1 - \frac{1}{x^2}\right) =
\lim_{x \to \infty} \left(1 + \frac{1}{x} - \frac{1}{x^2} - \frac{1}{x^3}\right) =
1 + 0 - 0 - 0 = \boxed{1}
\]
	
	
			\subsection{}
	
\[
\begin{array}{rcl}
	\lim_{x \to 0} \frac{\sqrt{x+1}-1}{x} 
	& = & \lim_{x \to 0} \frac{\sqrt{x+1}-1}{x} \cdot \frac{\sqrt{x+1}+1}{\sqrt{x+1}+1} \\
	& = & \lim_{x \to 0} \frac{(x+1) - 1}{x(\sqrt{x+1}+1)} \\
	& = & \lim_{x \to 0} \frac{x}{x(\sqrt{x+1}+1)} \\
	& = & \lim_{x \to 0} \frac{1}{\sqrt{x+1}+1} \\
	& = & \frac{1}{\sqrt{0+1}+1} \\
	& = & \frac{1}{2} = \boxed{\frac{1}{2}}
\end{array}
\]


			\subsection{}

\[
\begin{array}{rcl}
	\lim_{x \to 4} \frac{\sqrt{2x+1}-3}{\sqrt{x}-2} 
	& = & \lim_{x \to 4} \frac{\sqrt{2x+1}-3}{\sqrt{x}-2} \cdot \frac{\sqrt{2x+1}+3}{\sqrt{2x+1}+3} \\ 
	& = & \lim_{x \to 4} \frac{(2x+1) - 9}{(\sqrt{x}-2)(\sqrt{2x+1}+3)} \\ 
	& = & \lim_{x \to 4} \frac{2x - 8}{(\sqrt{x}-2)(\sqrt{2x+1}+3)} \\ 
	& = & \lim_{x \to 4} \frac{2(\sqrt{x}-2)(\sqrt{x}+2)}{(\sqrt{x}-2)(\sqrt{2x+1}+3)} \\ 
	& = & \lim_{x \to 4} \frac{2(\sqrt{x}+2)}{\sqrt{2x+1}+3} \\ 
	& = & \frac{2(\sqrt{4}+2)}{\sqrt{2 \cdot 4 + 1}+3} \\ 
	& = & \frac{2(2+2)}{\sqrt{9}+3} \\ 
	& = & \frac{2 \cdot 4}{3 + 3} \\ 
	& = & \frac{8}{6} = \frac{4}{3} = \boxed{\frac{4}{3}}
\end{array}
\]


			\section{}
			
						\subsection{}
\[
\begin{array}{rcl}
	\lim_{x \to 0} \frac{1 - \cos(2x)}{x \sin x} 
	& = & \lim_{x \to 0} \frac{1 - (2\cos^2(x) - 1)}{x \sin x} \\ 
	& = & \lim_{x \to 0} \frac{2(1 - \cos^2(x))}{x \sin x} \\ 
	& = & \lim_{x \to 0} \frac{2\sin^2(x)}{x \sin x} \\ 
	& = & \lim_{x \to 0} \frac{2\sin(x)}{x} \\ 
	& = & 2 \cdot \lim_{x \to 0} \frac{\sin(x)}{x} \\ 
	& = & 2 \cdot 1 \\ 
	& = & 2
\end{array}
\]



						\subsection{}
\[
\begin{array}{rcl}
	\lim_{x \to 0} x \cdot \cot(x) 
	& = & \lim_{x \to 0} x \cdot \frac{\cos(x)}{\sin(x)} \\ 
	& = & \lim_{x \to 0} \frac{x \cos(x)}{\sin(x)} \\ 
	& = & \lim_{x \to 0} \frac{x}{\sin(x)} \cdot \cos(x) \\ 
	& = & \lim_{x \to 0} \frac{1}{\frac{\sin(x)}{x}} \cdot \cos(x) \\ 
	& = & \frac{1}{1} \cdot \cos(0) \\ 
	& = & 1 \cdot 1 \\ 
	& = & 1
\end{array}
\]
						\subsection{}
\[
\begin{array}{rcl}
	\lim_{x \to 0} \frac{\arctan(x)}{x} 
	& = & \lim_{t \to 0} \frac{t}{\tan(t)} \\
	& = & 1
\end{array}
\]
						\subsection{}
\[
\begin{array}{rcl}
	\lim_{x \to \frac{\pi}{2}} \frac{\cos x}{x - \frac{\pi}{2}} 
	& = & \lim_{x \to \frac{\pi}{2}} \frac{-\sin x}{1} \quad \text{(Applying L'HÃ´pital's Rule)} \\
	& = & -\sin\left(\frac{\pi}{2}\right) \\
	& = & -1.
\end{array}
\]
					\section{}

						\subsection{}

\[
\begin{array}{rcl}
	\lim_{x \to \infty} \left( \frac{x}{1+x} \right)^x 
	& = & \lim_{x \to \infty} e^{x \ln\left( \frac{x}{1+x} \right)} \\
	& = & \lim_{x \to \infty} e^{x \left( \ln x - \ln(1+x) \right)} \\
	& = & \lim_{x \to \infty} e^{x \left( \ln x - \left( \ln x + \frac{1}{x} \right) \right)} \\
	& = & \lim_{x \to \infty} e^{-1} \\
	& = & \frac{1}{e}.
\end{array}
\]


						\subsection{}
\[
\begin{array}{rcl}
	\lim_{x \to \infty} \left(1 - \frac{1}{x} \right)^{kx} 
	& = & \lim_{x \to \infty} \left[\left(1 - \frac{1}{x}\right)^{x}\right]^k \\
	& = & \left(\lim_{x \to \infty} \left(1 - \frac{1}{x}\right)^{x}\right)^{k} \quad \text{(using the known limit)} \\
	& = & (e^{-1})^{k} \\
	& = & e^{-k}.
\end{array}
\]


\section{}
						\subsection{}
\[
\begin{array}{rcl}
	\lim_{x \to 1} \frac{1 - x^2}{1 - x} 
	& = & \lim_{x \to 1} \frac{(1 - x)(1 + x)}{1 - x} \quad \text{(factoring the numerator)} \\
	& = & \lim_{x \to 1} (1 + x) \quad \text{(canceling the common factor)} \\
	& = & 1 + 1 \\
	& = & 2.
\end{array}
\]
					\section{}
						\subsection{}
\[
\begin{array}{rcl}
	\lim_{x \to \infty} \frac{x^2 - 2x + 1}{x^2 + 1} 
	& = & \lim_{x \to \infty} \frac{x^2(1 - \frac{2}{x} + \frac{1}{x^2})}{x^2(1 + \frac{1}{x^2})} \quad \text{(factoring out } x^2 \text{)} \\
	& = & \lim_{x \to \infty} \frac{1 - \frac{2}{x} + \frac{1}{x^2}}{1 + \frac{1}{x^2}} \quad \text{(canceling } x^2 \text{)} \\
	& = & \frac{1 - 0 + 0}{1 + 0} \quad \text{(as } x \to \infty \text{)} \\
	& = & 1.
\end{array}
\]

						\subsection{}
\[
\begin{array}{rcl}
	\lim_{x \to \infty} \frac{x^2 - 1}{2x^2 + x + 1} 
	& = & \lim_{x \to \infty} \frac{x^2(1 - \frac{1}{x^2})}{x^2(2 + \frac{1}{x} + \frac{1}{x^2})} \quad \text{(factoring out } x^2 \text{)} \\
	& = & \lim_{x \to \infty} \frac{1 - \frac{1}{x^2}}{2 + \frac{1}{x} + \frac{1}{x^2}} \quad \text{(canceling } x^2 \text{)} \\
	& = & \frac{1 - 0}{2 + 0 + 0} \quad \text{(as } x \to \infty \text{)} \\
	& = & \frac{1}{2}.
\end{array}
\]


\subsection{}
\[
\begin{array}{rcl}
	\lim_{x \to \infty} \frac{100x^2 + 1}{2x^3 - 100x} 
	& = & \lim_{x \to \infty} \frac{x^2(100 + \frac{1}{x^2})}{x^3(2 - \frac{100}{x^2})} \quad \text{(factoring out } x^2 \text{ and } x^3 \text{)} \\
	& = & \lim_{x \to \infty} \frac{100 + \frac{1}{x^2}}{x(2 - \frac{100}{x^2})} \quad \text{(simplifying)} \\
	& = & \frac{100 + 0}{\infty(2 - 0)} \quad \text{(as } x \to \infty \text{)} \\
	& = & 0.
\end{array}
\]

\subsection{}
\[
\begin{array}{rcl}
	\lim_{x \to 1} \left(\frac{1}{1-x} - \frac{3}{1-x^3}\right) 
	& = & \lim_{x \to 1} \left(\frac{1}{1-x} - \frac{3}{(1-x)(1+x+x^2)}\right) \quad \text{(using } 1 - x^3 = (1-x)(1+x+x^2)\text{)} \\
	& = & \lim_{x \to 1} \frac{(1+x+x^2) - 3}{(1-x)(1+x+x^2)} \\
	& = & \lim_{x \to 1} \frac{x^2 + x - 2}{(1-x)(1+x+x^2)} \\
	& = & \lim_{x \to 1} \frac{(x - 1)(x + 2)}{(1 - x)(1 + x + x^2)} \\
	& = & \lim_{x \to 1} \frac{-(1-x)(x + 2)}{(1 - x)(1 + x + x^2)} \\
	& = & \lim_{x \to 1} \frac{-(x + 2)}{1 + x + x^2} \\
	& = & \frac{-(1 + 2)}{1 + 1 + 1} \\
	& = & \frac{-3}{3} \\
	& = & -1.
\end{array}
\]
\subsection{}
\[
\begin{array}{rcl}
	\lim_{x \to \infty} \left(\sqrt{x^2+x} - \sqrt{x^2-x} \right) 
	& = & \lim_{x \to \infty} \left(\sqrt{x^2+x} - \sqrt{x^2-x} \right) \cdot \frac{\sqrt{x^2+x} + \sqrt{x^2-x}}{\sqrt{x^2+x} + \sqrt{x^2-x}} 
	 \\ \quad \text{(multiply by the conjugate)} \\
	& = & \lim_{x \to \infty} \frac{(x^2+x) - (x^2-x)}{\sqrt{x^2+x} + \sqrt{x^2-x}} \\
	& = & \lim_{x \to \infty} \frac{2x}{\sqrt{x^2+x} + \sqrt{x^2-x}} \\
	& = & \lim_{x \to \infty} \frac{2x}{\sqrt{x^2(1+\frac{1}{x})} + \sqrt{x^2(1-\frac{1}{x})}} \quad \text{(factor out } x^2\text{)} \\
	& = & \lim_{x \to \infty} \frac{2x}{x\left(\sqrt{1+\frac{1}{x}} + \sqrt{1-\frac{1}{x}}\right)} \quad \text{(cancel } x\text{)} \\
	& = & \lim_{x \to \infty} \frac{2}{\sqrt{1+\frac{1}{x}} + \sqrt{1-\frac{1}{x}}} \\
	& = & \frac{2}{\sqrt{1+0} + \sqrt{1-0}} \quad \text{(as } x \to \infty\text{)} \\
	& = & \frac{2}{1 + 1} \\
	& = & 1.
\end{array}
\]


\end{document}
